spc/SProp.v
@@ -3,104 +3,166 @@ From sflib Require Import sflib.
 From iris Require Import bi.big_op.
 From iris Require base_logic.lib.invariants.
 From Coq Require Import Program Arith.
-Require Import PCM IProp IPM RobustIndexedInvariants.
+Require Import Coqlib PCM PCMAux IProp IPM.
+Require Import PropExtensionality.
 
-Local Notation level := nat.
+Module HRA.
 
-Module sAtom.
-
-  Section SATOM.
-
-  Context `{Σ : GRA.t}.
+  Section HRA.
   
-  Class t: Type := mk {
-    car:> forall (sProp: Type), Type;
-    interp: forall {sProp} (itp: sProp -> iProp), car sProp -> iProp;
+  Class t := __HRA_INTERNAL : GRA.t.
+
+  Class subG (Γ: t) (Σ: GRA.t) : Type := {
+    subG_map: nat -> nat;
+    subG_prf: forall i, Σ (subG_map i) = Γ i;
   }.
 
-  Instance empty: t := {
-      car sProp := sProp;
-      interp sProp itp := itp;
+  Coercion subG_map: subG >-> Funclass.
+
+  Context `{Γ: t}.
+  Context `{Σ: GRA.t}.
+  Context `{sub: @subG Γ Σ}.
+  
+  Global Program Instance embed (i:nat) : @GRA.inG (Γ i) Σ := {
+      inG_id := sub i;
     }.
-
-  Instance pointwise {D} (M: D -> t): t := {
-      car sProp := { d & (M d).(car) sProp };
-      interp sProp itp p := (M (projT1 p)).(interp) itp (projT2 p);
-    }.
-
-  End SATOM.
+  Next Obligation. i. symmetry. apply HRA.subG_prf. Qed.
   
-End sAtom.
-
-Coercion sAtom.car: Sortclass >-> Sortclass.
-
-Module GAtom.
-
-  Section GATOM.
-  
-  Context `{Σ : GRA.t}.
-  
-  Class t: Type := __GATOM_INTERNAL : (nat -> sAtom.t).
-  
-  Class inG (PB: sAtom.t) (α: t) := InG {
-    inG_id: nat;
-    inG_prf: PB = α inG_id;
-  }
-  .
-  
-  Class subG (α0 α1: t) := SubG i : { j | α0 i = α1 j }.
-
-  Definition of_list (RAs: list sAtom.t): t := fun n => List.nth n RAs (sAtom.empty).
-
-  Definition to_sAtom (α: t): sAtom.t := sAtom.pointwise α.
-
-  Coercion to_sAtom: t >-> sAtom.t.
-
-  Let cast_pb {A B: sAtom.t} (EQ: A = B) {sProp} (a: A.(sAtom.car) sProp): B.(sAtom.car) sProp :=
-    eq_rect_r (λ A0, A0.(sAtom.car) sProp → B.(sAtom.car) sProp) id EQ a.
-
-  Definition embed {A α} `{@inG A α} {sProp} (a: A.(sAtom.car) sProp): α.(sAtom.car) sProp :=
-    existT inG_id (cast_pb inG_prf a).
-
-  Lemma embed_interp
-        A α
-        `{@inG A α}
-        sProp itp (a: A.(sAtom.car) sProp)
-    :
-    α.(sAtom.interp) itp (embed a) = A.(sAtom.interp) itp a.
-  Proof.
-    destruct H. subst. eauto.
+  Global Program Instance in_subG `{M: URA.t} `{emb: @GRA.inG M Γ} : @GRA.inG M Σ := {
+      inG_id := sub.(subG_map) emb.(GRA.inG_id);
+      }.
+  Next Obligation.
+    i. destruct emb. subst. destruct sub. ss.
   Qed.
-
-  End GATOM.
-
-End GAtom.
   
-Coercion GAtom.to_sAtom: GAtom.t >-> sAtom.t.
-Coercion GAtom.embed: sAtom.car >-> sAtom.car.
+  (* Definition embed `{Γ: GRA.t} `{Σ: GRA.t} `{m: @subG Γ Σ} (r: Σ) : Γ := *)
+  (*   fun i => eq_rect _ (@URA.car) (r (m i)) _ (m.(subG_prf) i). *)
 
-Global Opaque GAtom.to_sAtom.
+  (* Lemma embed_wf `{Γ: GRA.t} `{Σ: GRA.t} `{m: @subG Γ Σ} (r: Σ) *)
+  (*     (WF: URA.wf r): *)
+  (*   URA.wf (embed r). *)
+  (* Proof. *)
+  (*   Local Transparent GRA.to_URA. *)
+  (*   revert WF. unfold URA.wf, embed. unseal "ra". ss. *)
+  (*   i. specialize (WF (m k)). revert WF. *)
+  (*   rewrite <-(m.(subG_prf) k). ss. *)
+  (* Qed. *)
+
+  (* Lemma embed_extends `{Γ: GRA.t} `{Σ: GRA.t} `{m: @subG Γ Σ} (r0 r1: Σ) *)
+  (*     (EXT: URA.extends r0 r1): *)
+  (*   URA.extends (embed r0) (embed r1). *)
+  (* Proof. *)
+  (*   Local Transparent GRA.to_URA. *)
+  (*   rr in EXT. des. subst. exists (embed ctx). extensionality k. *)
+  (*   unfold embed, URA.add. unseal "ra". simpl. *)
+  (*   rewrite <-(m.(subG_prf) k). ss. *)
+  (* Qed. *)
+  
+  (* Program Definition lift `{Γ: GRA.t} `{Σ: GRA.t} `{m: @subG Γ Σ} (P: @iProp Γ): @iProp Σ := *)
+  (*   iProp_intro (fun r => P (embed r)) _. *)
+  (* Next Obligation. *)
+  (*   i. ss. eapply iProp_mono; eauto using embed_wf, embed_extends. *)
+  (* Qed. *)
+
+  (* Lemma iprop_extensionality `{Σ: GRA.t} (P Q: iProp) *)
+  (*     (EQ: iProp_pred P = iProp_pred Q): *)
+  (*   P = Q. *)
+  (* Proof. *)
+  (*   destruct P eqn: EQP. subst. *)
+  (*   destruct Q eqn: EQQ. subst. *)
+  (*   ss. subst. f_equal. eapply proof_irrelevance. *)
+  (* Qed. *)
+  
+  (* Lemma lift_ownM `{Γ: GRA.t} `{Σ: GRA.t} `{sub: @subG Γ Σ} {M: URA.t} {emb: @GRA.inG M Γ} (m: M): *)
+  (*   lift (@OwnM Γ M emb m) = @OwnM Σ M (in_subG sub emb) m. *)
+  (* Proof. *)
+  (*   Local Transparent GRA.to_URA. *)
+  (*   apply iprop_extensionality. ss. *)
+  (*   extensionality i. unfold OwnM, embed, Own, URA.extends. uiprop. *)
+  (*   destruct emb, sub. subst. *)
+  (*   rename i into r. apply propositional_extensionality. split; i; des. *)
+  (*   - exists (fun k => *)
+  (*               match Nat.eq_dec (subG_map0 inG_id) k with *)
+  (*               | left H => *)
+  (*                   eq_rect _ (fun k => @URA.car (Σ k)) *)
+  (*                   (eq_rect_r (@URA.car) (ctx inG_id) (subG_prf0 inG_id)) _ H *)
+  (*               | _ => r k *)
+  (*               end). *)
+  (*     extensionality k. ss. *)
+  (*     assert (EQ:= equal_f_dep H inG_id). clear H. *)
+  (*     unfold URA.add in *. unseal "ra". ss. *)
+  (*     unfold GRA.embed in *. ss. des_ifs; r_solve. ss. *)
+  (*     unfold URA.add in *. unseal "ra". unfold PCM.GRA.cast_ra. clear Heq. *)
+  (*     revert EQ. rewrite (UIP_refl _ _ e). ss. clear e. *)
+  (*     rewrite (UIP_refl _ _ e0). ss. clear e0. *)
+  (*     generalize (in_subG_obligation_1 Γ Σ (Γ inG_id)  *)
+  (*         {| subG_map := subG_map0; subG_prf := subG_prf0 |} *)
+  (*         {| GRA.inG_id := inG_id; GRA.inG_prf := eq_refl |}). *)
+  (*     generalize (subG_prf0 inG_id). ss. *)
+  (*     unfold eq_rect_r. i. rewrite (UIP _ _ _ (eq_sym e) e0). *)
+  (*     revert_until r. generalize (subG_map0 inG_id) as j. *)
+  (*     intros j. generalize (r j) as r'. clear r. *)
+  (*     generalize (Σ j) as A. clear j. clear Σ subG_prf0 subG_map0. *)
+  (*     i. subst. rewrite (UIP_refl _ _ e0). ss. *)
+  (*   - ss.       *)
+  (*     exists (fun k => *)
+  (*               match Nat.eq_dec inG_id k with *)
+  (*               | left H => eq_rect _ (@URA.car) (ctx (subG_map0 k)) _ (subG_prf0 k)  *)
+  (*               | _ => eq_rect _ (@URA.car) (r (subG_map0 k)) _ (subG_prf0 k) *)
+  (*               end). *)
+  (*     extensionality k. *)
+  (*     assert (EQ:= equal_f_dep H (subG_map0 inG_id)). clear H. *)
+  (*     unfold URA.add in *. unseal "ra". ss. *)
+  (*     unfold GRA.embed in *. ss. des_ifs; r_solve. ss. *)
+  (*     unfold URA.add in *. unseal "ra". clear Heq e. *)
+  (*     revert EQ. unfold PCM.GRA.cast_ra. *)
+  (*     rewrite (UIP_refl _ _ e0). ss. clear e0. *)
+  (*     generalize (in_subG_obligation_1 Γ Σ (Γ k) *)
+  (*         {| subG_map := subG_map0; subG_prf := subG_prf0 |} *)
+  (*         {| GRA.inG_id := k; GRA.inG_prf := eq_refl |}). ss. *)
+  (*     generalize (subG_prf0 k). generalize (subG_map0 k). *)
+  (*     intros j. generalize (r j) as r'. clear r. revert m. *)
+  (*     generalize (ctx j). clear ctx. *)
+  (*     generalize (Σ j) as A. clear j. i. subst. *)
+  (*     rewrite (UIP_refl _ _ e0). ss. *)
+  (* Qed. *)
+
+  End HRA.
+  
+End HRA.
+
+Coercion HRA.subG_map: HRA.subG >-> Funclass.
+
+Module sAtom.
+  
+  Class t: Type := car : forall (sProp: Type), Type.
+
+End sAtom.
 
 Module sType.
 
   Class t : Type := mk {
-    car:> Type;
-    interp: car -> forall sProp: Type, Type                        
+    car: Type;
+    interp: car -> forall sProp: Type, Type;
   }.
 
 End sType.
 
 Coercion sType.car: sType.t >-> Sortclass.
 
+Local Notation level := nat.
+
 Module sProp.
 
-  Section SPROP.
+  Section SYNTAX.
 
   Context `{τ: sType.t}.
-  Context `{α: GAtom.t}.
+  Context `{Γ: HRA.t}.
+  Context `{A : Type}.
 
   Inductive t {sProp : Type} : Type :=
-  | atom (a : α.(sAtom.car) sProp) : t
+  | ownm i (r : Γ i) : t
+  | atom (a : A) : t
   | lift (p : sProp) : t
   | pure (P : Prop) : t
   | and (p q : t) : t
@@ -116,125 +178,174 @@ Module sProp.
   | upd (p : t) : t
   .
 
+  End SYNTAX.
+
+  Section SPROP.
+
+  Context `{τ: sType.t}.
+  Context `{Γ: HRA.t}.
+  Context `{As : sAtom.t}.
+  
   Fixpoint _sProp (n : level) : Type :=
     match n with
     | O => Empty_set
-    | S m => @t (_sProp m)
+    | S m => @t _ _ (As (_sProp m)) (_sProp m) 
     end.
 
   Definition sProp (n : level) : Type := _sProp (S n).
 
   Definition affinely {n} (p : sProp n) : sProp n :=
     and empty p.
-  
-  Fixpoint _interp n : _sProp n -> iProp :=
-    match n with
-    | O => fun _ => ⌜False⌝%I
-    | S m => fix _interp_sProp_aux (syn : t) : iProp :=
-      match syn with
-      | atom a => α.(sAtom.interp) (_interp m) a
-      | lift p => _interp m p
-      | pure P => Pure P
-      | and p q => And (_interp_sProp_aux p) (_interp_sProp_aux q)
-      | or p q => Or (_interp_sProp_aux p) (_interp_sProp_aux q)
-      | impl p q => Impl (_interp_sProp_aux p) (_interp_sProp_aux q)
-      | univ ty p => Univ (fun (x : τ.(sType.interp) ty (_sProp m)) => _interp_sProp_aux (p x))
-      | ex ty p => Ex (fun (x : τ.(sType.interp) ty (_sProp m)) => _interp_sProp_aux (p x))
-      | empty => Emp
-      | sepconj p q => Sepconj (_interp_sProp_aux p) (_interp_sProp_aux q)
-      | wand p q => Wand (_interp_sProp_aux p) (_interp_sProp_aux q)
-      | persistently p => Persistently (_interp_sProp_aux p)
-      | plainly p => IProp.Plainly (_interp_sProp_aux p)
-      | upd p => Upd (_interp_sProp_aux p)
-      end
+
+  Fixpoint liftn n {m} (p: sProp m) : sProp (n+m) :=
+    match n return sProp (n+m) with
+    | 0 => p
+    | S n' => lift (liftn n' p)
     end.
-
-    Definition interp n : sProp n -> iProp := _interp (S n).
-
+  
   End SPROP.
 
 End sProp.
 
-Section RED.
+Module SAtom.
+
+  Section SATOM.
 
   Context `{τ: sType.t}.
-  Context `{α: GAtom.t}.
+  Context `{Γ: HRA.t}.
+  Context `{As: sAtom.t}.
+  Context `{Σ: GRA.t}.
+    
+  Class t : Type := interp :
+      forall (n:level), As (sProp._sProp n) -> iProp.
+
+  End SATOM.
+  
+End SAtom.
+
+Module sPropI.
+
+  Section INTERP.
+
+  Context `{α: SAtom.t}.
+  Context `{sub: @HRA.subG Γ Σ}.
 
   Import sProp.
 
+  Fixpoint _interp n : _sProp n -> iProp :=
+    match n with
+    | O => fun _ => ⌜False⌝%I
+    | S m => fix _interp_aux (syn : _sProp (S m)) : iProp :=
+      match syn with
+      | ownm i a => OwnM a        
+      | atom a => α m a
+      | lift p => _interp m p
+      | pure P => Pure P
+      | and p q => And (_interp_aux p) (_interp_aux q)
+      | or p q => Or (_interp_aux p) (_interp_aux q)
+      | impl p q => Impl (_interp_aux p) (_interp_aux q)
+      | univ ty p => Univ (fun x => _interp_aux (p x))
+      | ex ty p => Ex (fun x => _interp_aux (p x))
+      | empty => Emp
+      | sepconj p q => Sepconj (_interp_aux p) (_interp_aux q)
+      | wand p q => Wand (_interp_aux p) (_interp_aux q)
+      | persistently p => Persistently (_interp_aux p)
+      | plainly p => IProp.Plainly (_interp_aux p)
+      | upd p => Upd (_interp_aux p)
+      end
+    end.
+
+  Definition interp n : sProp n -> iProp := _interp (S n).
+
+  End INTERP.
+  
+End sPropI.
+
+Section RED.
+
+  Context `{α: SAtom.t}.
+  Context `{sub: @HRA.subG Γ Σ}.
+
+  Import sProp.
+  Import sPropI.
+
+  Lemma red_sem_ownm n i a :
+    interp n (ownm i a) = OwnM a.
+  Proof. reflexivity. Qed.
+  
   Lemma red_sem_atom n a :
-    interp n (atom a) = α.(sAtom.interp) (_interp n) a.
-  Proof. ss. Qed.
+    interp n (atom a) = α n a.
+  Proof. reflexivity. Qed.
 
   Lemma red_sem_lift_0 p :
     interp 0 (lift p) = ⌜False⌝%I.
-  Proof. ss. Qed.
+  Proof. reflexivity. Qed.
 
   Lemma red_sem_lift n p :
-    interp (S n) (lift p) = interp n p.
-  Proof. ss. Qed.
+    interp n (lift p) = _interp n p.
+  Proof. reflexivity. Qed.
 
   Lemma red_sem_pure n P :
     interp n (pure P) = ⌜P⌝%I.
-  Proof. ss. Qed.
+  Proof. reflexivity. Qed.
 
   Lemma red_sem_and n p q :
     interp n (and p q) = (interp n p ∧ interp n q)%I.
-  Proof. ss. Qed.
+  Proof. reflexivity. Qed.
 
   Lemma red_sem_or n p q :
     interp n (or p q) = (interp n p ∨ interp n q)%I.
-  Proof. ss. Qed.
+  Proof. reflexivity. Qed.
 
   Lemma red_sem_impl n p q :
     interp n (impl p q) = (interp n p → interp n q)%I.
-  Proof. ss. Qed.
+  Proof. reflexivity. Qed.
 
   Lemma red_sem_univ n ty p :
-    interp n (univ ty p) = (∀ (x : τ.(sType.interp) ty (_sProp n)), interp n (p x))%I.
-  Proof. ss. Qed.
+    interp n (univ ty p) = (∀ x, interp n (p x))%I.
+  Proof. reflexivity. Qed.
 
   Lemma red_sem_ex n ty p :
-    interp n (ex ty p) = (∃ (x : τ.(sType.interp) ty (_sProp n)), interp n (p x))%I.
-  Proof. ss. Qed.
+    interp n (ex ty p) = (∃ x, interp n (p x))%I.
+  Proof. reflexivity. Qed.
 
   Lemma red_sem_empty n :
     interp n empty = emp%I.
-  Proof. ss. Qed.
+  Proof. reflexivity. Qed.
   
   Lemma red_sem_sepconj n p q :
     interp n (sepconj p q) = (interp n p ∗ interp n q)%I.
-  Proof. ss. Qed.
+  Proof. reflexivity. Qed.
 
   Lemma red_sem_wand n p q :
     interp n (wand p q) = (interp n p -∗ interp n q)%I.
-  Proof. ss. Qed.
+  Proof. reflexivity. Qed.
 
   Lemma red_sem_persistently n p :
     interp n (persistently p) = (<pers> interp n p)%I.
-  Proof. ss. Qed.
+  Proof. reflexivity. Qed.
 
   Lemma red_sem_plainly n p :
     interp n (plainly p) = (IProp.Plainly (interp n p))%I.
-  Proof. ss. Qed.
+  Proof. reflexivity. Qed.
 
   Lemma red_sem_upd n p :
     interp n (upd p) = (#=> interp n p)%I.
-  Proof. ss. Qed.
+  Proof. reflexivity. Qed.
 
   Lemma red_sem_affinely n p :
     interp n (affinely p) = (<affine> interp n p)%I.
-  Proof. ss. Qed.
+  Proof. reflexivity. Qed.
 
   Lemma red_sem_intuitionistically n p :
     interp n (affinely (persistently p)) = (□ interp n p)%I.
-  Proof. ss. Qed.
+  Proof. reflexivity. Qed.
 
 End RED.
 
-Global Opaque sProp.interp.
+Global Opaque sPropI.interp.
 
-(** Simple sProp reduction tactics. *)
+(* Simple sProp reduction tactics. *)
 Ltac red_sem_binary_once := (try rewrite ! @red_sem_sepconj;
                              try rewrite ! @red_sem_and;
                              try rewrite ! @red_sem_or;
@@ -243,6 +354,7 @@ Ltac red_sem_binary_once := (try rewrite ! @red_sem_sepconj;
                             ).
 
 Ltac red_sem_unary_once := (try rewrite ! @red_sem_atom;
+                            try rewrite ! @red_sem_ownm;
                             try rewrite ! @red_sem_lift;
                             try rewrite ! @red_sem_pure;
                             try rewrite ! @red_sem_univ;
@@ -267,6 +379,7 @@ Ltac red_sem_binary_once_every := (try rewrite ! @red_sem_sepconj in *;
                                   ).
 
 Ltac red_sem_unary_once_every := (try rewrite ! @red_sem_atom in *;
+                                  try rewrite ! @red_sem_ownm in *;
                                   try rewrite ! @red_sem_lift in *;
                                   try rewrite ! @red_sem_pure in *;
                                   try rewrite ! @red_sem_univ in *;
@@ -318,3 +431,82 @@ Notation "∃'" := (f_exist _) (only parsing) : sProp_scope.
 Notation "∃ a .. z , P" := (f_exist _ (λ a, .. (f_exist _ (λ z, P%F)) ..)) : sProp_scope.
 Notation "'emp'" := (sProp.empty) : sProp_scope.
 
+(* Module TestLock. *)
+  
+(* Section TESTLOCK. *)
+
+(*   Context `{τ: sType.t}. *)
+(*   Context `{Σ : GRA.t}. *)
+  
+(*   Variant atm {sProp : Type} : Type := *)
+(*     | lock (p: sProp) : atm *)
+(*     | unlock (p: sProp) : atm *)
+(*   . *)
+  
+(*   Instance t : SAtom.t := { *)
+(*     car sProp := @atm sProp; *)
+(*     interp α n itp p := *)
+(*         match p with *)
+(*         | lock q => itp q -∗ itp q *)
+(*         | unlock q => itp q ∗ itp q *)
+(*         end%I *)
+(*   }. *)
+  
+(* End TESTLOCK. *)
+
+(* End TestLock. *)
+
+(* Require Import RobustIndexedInvariants. *)
+
+(* Module TestOwnI. *)
+  
+(* Section TestOwnI. *)
+
+(*   Context `{τ: sType.t}. *)
+(*   Context `{Σ: GRA.t}. *)
+(*   Context `{@GRA.inG OwnEsRA Σ}. *)
+(*   Context `{@GRA.inG (OwnIsRA sProp.sProp) Σ}. *)
+
+(*   Definition xxx (u: positive) (n: nat) (i: positive) : sProp.sProp 0 := *)
+(*     (⟨∃ p: iProp, p -∗ OwnI u n i ⟨OwnE u n ∅⟩⟩)%F. *)
+
+(*   Check (sPropSem.interp 0 (xxx 1 0 1)). *)
+(*   Check (OwnI 1 0 1 ⟨OwnE 1 0 ∅⟩). *)
+
+(*   Check (∃ p: iProp, p -∗ False)%I. *)
+  
+(*   Lemma foo: sPropSem.interp 0 (xxx 1 0 1) = OwnI 1 0 1 ⟨OwnE 1 0 ∅⟩. *)
+(*     reflexivity. *)
+(*   Qed.   *)
+  
+  
+(*   (* Context `{α: GAtom.t}. *) *)
+   
+(*   (* Variant atom {sProp : Type} : Type := *) *)
+(*   (* | owni (u: positive) (i : positive) (p : sProp.t (sProp:=sProp)) *) *)
+(*   (* . *) *)
+
+(*   (* Context `{@GRA.inG (OwnIsRA sProp) Σ}. *) *)
+  
+(*   (* Program Instance t : SAtom.t := { *) *)
+(*   (*   car sProp := @atom sProp; *) *)
+(*   (* }. *) *)
+(*   (* Next Obligation. *) *)
+(*   (*   intros. destruct X. *) *)
+(*   (*   Set Printing All. *) *)
+(*   (*   exact (@OwnI _ sProp.sProp _ u n i p). *) *)
+  
+(*   (*   interp α n itp p := *) *)
+(*   (*     match p with *) *)
+(*   (*     | owni u i p => @OwnI _ sProp.sProp _ u _ i p *) *)
+(*   (*     end *) *)
+(*   (* }. *) *)
+
+
+  
+  
+
+
+(* End TestOwnI. *)
+
+(* End TestOwnI. *)
